removed go

RunTime/src/Formalization.lean
@@ -1,49 +1,45 @@
-import data.list.sort
+import data.list.sort tactic
 
 variables {α : Type} (r : α → α → Prop) [decidable_rel r]
 local infix ` ≼ ` : 50 := r
 
 namespace counting
 
-@[simp] def go_oi (h : α) (p : list α × ℕ) : (list α × ℕ) := (h :: p.fst, p.snd + 1)
--- | (l, n) := (b :: l, n + 1)
-
--- the second value in the output is the number of comparisons made
 @[simp] def ordered_insert (a : α) : list α → (list α × ℕ)
 | []       := ([a], 0)
-| (h :: t) := if a ≼ h then (a :: h :: t, 0)
-                       -- else go_oi h (ordered_insert t)
+| (h :: t) := if a ≼ h then (a :: h :: t, 1)
                        else let (l', n) := ordered_insert t in (h :: l', n + 1)
-
--- @[simp] def go_is (p₁ : (list α × ℕ)) : (list α × ℕ) :=
 
 @[simp] def insertion_sort : list α → (list α × ℕ)
 | [] := ([], 0)
--- | (h :: t) := go_is (insertion_sort t)
 | (h :: t) := let (l', n) := (insertion_sort t) , (l'', m) := ordered_insert r h l'
               in (l'', n + m)
 
--- @[simp] def smaller_prefix (a : α) (l : list α) : ℕ := (list.take_while (λ m , m ≼ a) l).length
 @[simp] def smaller_prefix (a : α) : list α → ℕ
 | []       := 0
 | (h :: t) := if a ≼ h then 0 else 1 + smaller_prefix t
 
 end counting
 
-theorem ordered_insert_linear (a : α) : ∀ l : list α, (counting.ordered_insert r a l).snd ≤ l.length
-| [] := by simp
-| (h :: t) :=
+theorem ordered_insert_linear (a : α) : ∀ l : list α, (counting.ordered_insert r a l).snd ≤ l.length :=
 begin
-  simp,
-  split_ifs,
+  intro l,
+  induction l,
   { simp, },
-  {  }
+  { simp, split_ifs,
+    { simp, },
+    { cases (counting.ordered_insert r a l_tl),
+      unfold counting.ordered_insert,
+      simp,
+      exact l_ih,
+    }
+  }
 end
 
 theorem ordered_insert_identification (a : α) : ∀ l : list α,
   (counting.ordered_insert r a l).fst = list.ordered_insert r a l := sorry
 
-theorem counting_comparisons_oi (a : α) : ∀ l : list α,
+theorem counting_comparisons_ordered_insertion (a : α) : ∀ l : list α,
   (counting.ordered_insert r a l).snd = counting.smaller_prefix (≼) a l
 | []       := by simp
 | (h :: t) :=
@@ -56,9 +52,29 @@ begin
   }
 end
 
-theorem insertion_sort_quadratic : ∀ l : list α, (counting.insertion_sort r l).snd ≤ l.length * l.length
-| []       := by simp
-| (h :: t) := sorry
+#print counting.insertion_sort._match_1
+
+theorem insertion_sort_quadratic : ∀ l : list α, (counting.insertion_sort r l).snd ≤ (l.length * l.length) :=
+begin
+  intro l,
+  induction l,
+  { simp, },
+  { simp,
+    cases (counting.insertion_sort r l_tl) with sorted_tl ops,
+    unfold counting.insertion_sort,
+    have hh : (counting.ordered_insert r l_hd sorted_tl).snd ≤
+       sorted_tl.length := ordered_insert_linear r l_hd sorted_tl,
+    cases (counting.ordered_insert r l_hd sorted_tl),
+    unfold counting.insertion_sort,
+    have same_lengths : sorted_tl.length = l_tl.length :=
+    begin
+      induction sorted_tl,
+      { sorry },
+      { sorry }
+    end,
+    linarith,
+  }
+end
 
 theorem insertion_sort_identification (a : α) : ∀ l : list α,
   (counting.insertion_sort r l).fst = list.insertion_sort r l := sorry
